common/CallconvAlgebra.v
@@ -28,48 +28,66 @@ Require Import InjectFootprint.
   refined by the calling convention [cc'], meaning that any
   [cc']-simulation is also a [cc]-simulation. *)
 
-Definition ccref {li1 li2} (cc cc': callconv li1 li2) :=
-  forall w se1 se2 q1 q2,
-    match_senv cc w se1 se2 ->
-    match_query cc w q1 q2 ->
+Definition ccref_query_reply {li1 li2} (cc cc': callconv li1 li2)
+  {sk1 sk2} (path path': Genv.skel_path sk1 sk2) :=
+  forall w se1 se2, match_senv cc w path se1 se2 ->
+    forall q1 q2, match_query cc w q1 q2 ->
     exists w',
-      match_senv cc' w' se1 se2 /\
+      match_senv cc' w' path' se1 se2 /\
       match_query cc' w' q1 q2 /\
-      forall r1 r2,
-        match_reply cc' w' r1 r2 ->
+      forall r1 r2, match_reply cc' w' r1 r2 ->
         match_reply cc w r1 r2.
+
+Record ccref_component {li1 li2} (cc cc': callconv li1 li2): Type :=
+  Ccref {
+    (* skel_path_ref {sk1 sk2}: *)
+    (*   { skel_path' | @valid_skel _ _ cc' sk1 sk2 skel_path' } -> *)
+    (*   { skel_path | @valid_skel _ _ cc sk1 sk2 skel_path }; *)
+    path_ref {sk1 sk2}:
+      Genv.skel_path sk1 sk2 -> option (Genv.skel_path sk1 sk2);
+    ccref_prop {sk1 sk2}:
+      forall (path': Genv.skel_path sk1 sk2),
+        valid_skel cc' path' ->
+        exists path, path_ref path' = Some path /\
+                valid_skel cc path /\
+                ccref_query_reply cc cc' path path';
+  }.
+(* match_senv cc w (proj1_sig (skel_path_ref (exist _ path' H))) se1 se2 -> *)
+
+Definition ccref {li1 li2} (cc cc': callconv li1 li2) :=
+  inhabited (@ccref_component li1 li2 cc cc').
 
 Definition cceqv {li1 li2} (cc cc': callconv li1 li2) :=
   ccref cc cc' /\ ccref cc' cc.
 
-Global Instance ccref_preo li1 li2:
-  PreOrder (@ccref li1 li2).
-Proof.
-  split.
-  - intros cc w q1 q2 Hq.
-    eauto.
-  - intros cc cc' cc'' H' H'' w se1 se2 q1 q2 Hse Hq.
-    edestruct H' as (w' & Hse' & Hq' & Hr'); eauto.
-    edestruct H'' as (w'' & Hse'' & Hq'' & Hr''); eauto 10.
-Qed.
+(* Global Instance ccref_preo li1 li2: *)
+(*   PreOrder (@ccref li1 li2). *)
+(* Proof. *)
+(*   split. *)
+(*   - intros cc w q1 q2 Hq. *)
+(*     eauto. *)
+(*   - intros cc cc' cc'' H' H'' w se1 se2 se_path q1 q2 Hse Hq. *)
+(*     edestruct H' as (w' & Hse' & Hq' & Hr'); eauto. *)
+(*     edestruct H'' as (w'' & Hse'' & Hq'' & Hr''); eauto 10. *)
+(* Qed. *)
 
-Global Instance cceqv_equiv li1 li2:
-  Equivalence (@cceqv li1 li2).
-Proof.
-  split.
-  - intros cc.
-    split; reflexivity.
-  - intros cc1 cc2. unfold cceqv.
-    tauto.
-  - intros cc1 cc2 cc3 [H12 H21] [H23 H32].
-    split; etransitivity; eauto.
-Qed.
+(* Global Instance cceqv_equiv li1 li2: *)
+(*   Equivalence (@cceqv li1 li2). *)
+(* Proof. *)
+(*   split. *)
+(*   - intros cc. *)
+(*     split; reflexivity. *)
+(*   - intros cc1 cc2. unfold cceqv. *)
+(*     tauto. *)
+(*   - intros cc1 cc2 cc3 [H12 H21] [H23 H32]. *)
+(*     split; etransitivity; eauto. *)
+(* Qed. *)
 
-Global Instance ccref_po li1 li2:
-  PartialOrder (@cceqv li1 li2) (@ccref li1 li2).
-Proof.
-  firstorder.
-Qed.
+(* Global Instance ccref_po li1 li2: *)
+(*   PartialOrder (@cceqv li1 li2) (@ccref li1 li2). *)
+(* Proof. *)
+(*   firstorder. *)
+(* Qed. *)
 
 (** ** Relation to forward simulations *)
 
@@ -80,37 +98,43 @@ Global Instance open_fsim_ccref:
      forallr - @ liB1, forallr - @ liB2, ccref -->
      subrel).
 Proof.
-  intros liA1 liA2 ccA ccA' HA liB1 liB2 ccB ccB' HB sem1 sem2 [FS].
-  destruct FS as [index order match_states SKEL PROP WF].
+  intros liA1 liA2 ccA ccA' [HA] liB1 liB2 ccB ccB' [HB] sem1 sem2 [FS].
+  destruct FS as [index order match_states SKEL VSK PROP WF].
+  destruct HA as [SKREF1 HA]. destruct HB as [SKREF2 HB].
+  pose proof (HB' := HB).
+  specialize (HB _ _ _ VSK) as (path' & Hpath' & Hv' & Href).
   constructor.
   set (ms se1 se2 w' idx s1 s2 :=
          exists w : ccworld ccB,
            match_states se1 se2 w idx s1 s2 /\
-           match_senv ccB w se1 se2 /\
+           match_senv ccB w SKEL se1 se2 /\
            forall r1 r2, match_reply ccB w r1 r2 -> match_reply ccB' w' r1 r2).
-  eapply Forward_simulation with order ms; auto.
-  intros se1 se2 wB' Hse' Hse1.
+  eapply Forward_simulation with order ms path'; auto.
+  intros se1 se2 wB' Hse'. specialize (Href _ _ _ Hse').
   split.
   - intros q1 q2 Hq'.
-    destruct (HB wB' se1 se2 q1 q2) as (wB & Hse & Hq & Hr); auto.
-    eapply fsim_match_valid_query; eauto.
+    destruct (Href q1 q2) as (wB & Hse & Hq & Hr); auto.
+    erewrite fsim_match_valid_query; eauto.
   - intros q1 q2 s1 Hq' Hs1.
-    destruct (HB wB' se1 se2 q1 q2) as (wB & Hse & Hq & Hr); auto.
+    destruct (Href q1 q2) as (wB & Hse & Hq & Hr); auto.
     edestruct @fsim_match_initial_states as (i & s2 & Hs2 & Hs); eauto.
     exists i, s2. split; auto. exists wB; auto.
   - intros i s1 s2 r1 (wB & Hs & Hse & Hr') Hr1.
     edestruct @fsim_match_final_states as (r2 & Hr2 & Hr); eauto.
-  - intros i s1 s2 qA1 (wB & Hs & Hse & Hr') HqA1.
-    edestruct @fsim_match_external as (wA & qA2 & HqA2 & HqA & HseA & ?); eauto.
-    edestruct HA as (wA' & HseA' & HqA' & Hr); eauto.
+  - intros i s1 s2 qA1 (wB & Hs & Hse & Hr') HqA1 * HpathA'.
+    specialize (HA _ _ _ HpathA') as (pathA & HpathA & HvA & HrefA).
+    edestruct @fsim_match_external
+      as (wA & qA2 & HqA2 & HseA & HqA & HrA); eauto.
+    edestruct HrefA as (wA' & HseA' & HqA' & Hr); eauto.
     exists wA', qA2. intuition auto.
-    edestruct H as (i' & s2' & Hs2' & Hs'); eauto.
+    edestruct HrA as (i' & s2' & Hs2' & Hs'); eauto.
     exists i', s2'. split; auto. exists wB; eauto.
   - intros s1 t s1' Hs1' i s2 (wB & Hs & Hse & Hr').
     edestruct @fsim_simulation as (i' & s2' & Hs2' & Hs'); eauto.
     exists i', s2'. split; auto. exists wB; eauto.
 Qed.
 
+(*
 Global Instance open_bsim_ccref:
   Monotonic
     (@backward_simulation)
@@ -121,19 +145,19 @@ Proof.
   intros liA1 liA2 ccA ccA' HA liB1 liB2 ccB ccB' HB sem1 sem2 [FS].
   destruct FS as [index order match_states SKEL PROP WF].
   constructor.
-  set (ms se1 se2 w' idx s1 s2 :=
+  set (ms se1 se2 (se_path: Genv.symtbl_path se1 se2) w' idx s1 s2 :=
          exists w : ccworld ccB,
-           match_states se1 se2 w idx s1 s2 /\
-           match_senv ccB w se1 se2 /\
+           match_states se1 se2 se_path w idx s1 s2 /\
+           match_senv ccB w se_path /\
            forall r1 r2, match_reply ccB w r1 r2 -> match_reply ccB' w' r1 r2).
-  eapply Backward_simulation with order ms; auto.
-  intros se1 se2 wB' Hse' Hse1.
+  eapply Backward_simulation with order ms SKEL; auto.
+  intros se1 se2 se_path wB' Hse' Hse1.
   split.
   - intros q1 q2 Hq'.
-    destruct (HB wB' se1 se2 q1 q2) as (wB & Hse & Hq & Hr); auto.
+    destruct (HB wB' se1 se2 se_path q1 q2) as (wB & Hse & Hq & Hr); auto.
     eapply bsim_match_valid_query; eauto.
   - intros q1 q2 Hq'.
-    destruct (HB wB' se1 se2 q1 q2) as (wB & Hse & Hq & Hr); auto.
+    destruct (HB wB' se1 se2 se_path q1 q2) as (wB & Hse & Hq & Hr); auto.
     edestruct @bsim_match_initial_states as [EXIST MATCH]; eauto.
     split; auto.
     intros. edestruct MATCH as (s1' & Hs1' & i & Hs); eauto. 
@@ -154,23 +178,50 @@ Proof.
     edestruct @bsim_simulation as (i' & s1' & Hs1' & Hs'); eauto.
     exists i', s1'. split; auto. exists wB; eauto.
 Qed.
+*)
 
 (** * Properties of [cc_compose] *)
 
 (** Language interfaces and calling conventions form a category, with
   [cc_id] as the identity arrow and [cc_compose] as the composition. *)
 
+Definition g {sk1 sk2} (path: Genv.skel_path sk1 sk2):
+    option (Genv.skel_path sk1 sk2).
+Proof.
+  destruct path.
+  - refine None.
+  - refine None.
+  - destruct path1.
+    + refine (Some path2).
+    + refine None.
+    + refine None.
+Defined.
+
 Lemma cc_compose_id_left {li1 li2} (cc: callconv li1 li2):
   cceqv (cc_compose cc_id cc) cc.
 Proof.
   split.
-  - intros [[se2 [ ]] w] se1 se3 q1 q3 (Hse12 & Hse23) (q2 & Hq12 & Hq23).
-    simpl in *. subst.
-    exists w; intuition eauto.
-  - intros w se1 se2 q1 q2 Hse Hq.
+  - constructor.
+    set (f := fun {sk1 sk2} (path: Genv.skel_path sk1 sk2) =>
+                 Some (Genv.Compose (Genv.Same sk1) path)).
+    eapply Ccref with f.
+    intros sk1 sk2 path Hpath.
+    eexists. intuition eauto. repeat constructor; eauto.
+    intros [[se2 []] w] se1 se3 Hse q1 q3 (q2 & Hq12 & Hq23).
+    cbn in Hse. inv Hse. subst_dep.
+    inv SE12. inv Hq12.
+    exists w. intuition eauto.
+    econstructor. split; eauto. constructor.
+  - set (g := fun sk1 sk2 (path: Genv.skel_path sk1 sk2) => g path).
+    constructor.
+    eapply Ccref with g.
+    intros sk1 sk2 path' Hpath'. inv Hpath'.
+    cbn in H. destruct path12. 2-3: inv H.
+    exists path23. intuition eauto.
+    intros w se1 se2 Hse q1 q2 Hq.
     exists (se1, tt, w); repeat apply conj.
-    + cbn. eauto.
-    + cbn. eauto.
+    + cbn. constructor. constructor. eauto.
+    + cbn. eexists. split; eauto.
     + intros r1 r3 (r2 & Hr12 & Hr23); simpl in *.
       congruence.
 Qed.
