common/LanguageInterface.v
@@ -5,6 +5,16 @@ Require Import Memory.
 Require Import Globalenvs.
 Require Import Events.
 Require Import CKLR.
+Require Import Classical.       (* inj_pair2 *)
+
+Ltac subst_dep :=
+  subst;
+  lazymatch goal with
+    | H: existT ?P ?x _ = existT ?P ?x _ |- _ =>
+      apply inj_pair2 in H; subst_dep
+    | _ =>
+      idtac
+  end.
 
 (** * Semantic interface of languages *)
 
@@ -48,64 +58,77 @@ Definition li_wp :=
 Record callconv {li1 li2} :=
   mk_callconv {
     ccworld : Type;
-    match_senv: ccworld -> forall se1 se2, Genv.symtbl_path se1 se2 -> Prop;
+    valid_skel sk1 sk2: Genv.skel_path sk1 sk2 -> Prop;
+    match_senv:
+        ccworld -> forall sk1 sk2, Genv.skel_path sk1 sk2 ->
+        Genv.symtbl -> Genv.symtbl -> Prop;
     match_query: ccworld -> query li1 -> query li2 -> Prop;
     match_reply: ccworld -> reply li1 -> reply li2 -> Prop;
 
-    (* match_senv_local: *)
-    (* forall sk1 sk2 w path se1 se2, *)
-    (*   match_senv sk1 sk2 w path se1 se2 -> *)
-    (*   Genv.valid_stbls sk1 sk2 se1 se2; *)
+    match_senv_local:
+    forall sk1 sk2 w path se1 se2,
+      valid_skel _ _ path ->
+      match_senv w sk1 sk2 path se1 se2 ->
+      Genv.valid_stbls' sk1 sk2 se1 se2;
   }.
 
 Arguments callconv: clear implicits.
 Arguments match_senv {_ _} _ _ {_ _} _.
+Arguments valid_skel {_ _} _ {_ _} _.
 Delimit Scope cc_scope with cc.
 Bind Scope cc_scope with callconv.
 Local Obligation Tactic := cbn; eauto.
 
 (** ** Identity *)
 
-(* Inductive match_senv_id sk1 sk2: *)
-(*     skel_path sk1 sk2 -> Genv.symtbl -> Genv.symtbl -> Prop := *)
-(* | Match_senv_id_intro se (H: sk2 = sk1): *)
-(*     match_senv_id sk1 sk2 (Edge (same_skel_le _ _ H)) se se. *)
+Definition valid_skel_id {sk1 sk2} (path: Genv.skel_path sk1 sk2) : Prop.
+Proof.
+  destruct path.
+  - refine True.
+  - refine False.
+  - refine False.
+Defined.
 
 Program Definition cc_id {li}: callconv li li :=
   {|
     ccworld := unit;
-    match_senv w se1 se2 _ := se1 = se2;
+    valid_skel sk1 sk2 sk_path := valid_skel_id sk_path;
+    match_senv w _ _ _ se1 se2 := se1 = se2;
     match_query w := eq;
     match_reply w := eq;
   |}.
-(* Next Obligation. *)
-(*   intros. apply H. *)
-(* Qed. *)
+Next Obligation.
+  intros. subst.
+  (* FIXME: we need some [Genv.valid_for] in [match_senv] *)
+Admitted.
 
 Notation "1" := cc_id : cc_scope.
 
 (** ** Composition *)
 
+Inductive valid_skel_compose {li1 li2 li3} (cc12: callconv li1 li2)
+  (cc23: callconv li2 li3) sk1 sk3: Genv.skel_path sk1 sk3 -> Prop :=
+  | Valid_skel_compose_intro sk2 (path12: Genv.skel_path sk1 sk2)
+      (path23: Genv.skel_path sk2 sk3):
+      valid_skel cc12 path12 -> valid_skel cc23 path23 ->
+      valid_skel_compose cc12 cc23 _ _ (Genv.Compose path12 path23).
+
 Inductive match_senv_compose
-  {li1 li2 li3} (cc12: callconv li1 li2) (cc23: callconv li2 li3) {se1 se3}:
-    Genv.symtbl * ccworld cc12 * ccworld cc23 ->
-    Genv.symtbl_path se1 se3 -> Prop :=
-| Match_senv_compose_compose w12 w23 se2
-    (symtbl_path12: Genv.symtbl_path se1 se2) (symtbl_path23: Genv.symtbl_path se2 se3)
-    (SE12: match_senv cc12 w12 symtbl_path12)
-    (SE23: match_senv cc23 w23 symtbl_path23):
-    match_senv_compose cc12 cc23 (se2, w12, w23)
-      (Genv.Compose symtbl_path12 symtbl_path23)
-| Match_senv_compose_direct w12 w23 se2
-    (symtbl_path12: Genv.symtbl_path se1 se2) (symtbl_path23: Genv.symtbl_path se2 se3)
-    (SE12: match_senv cc12 w12 symtbl_path12)
-    (SE23: match_senv cc23 w23 symtbl_path23):
-    match_senv_compose cc12 cc23 (se2, w12, w23) (Genv.Direct (fun _ _ => True) _ _ I).
+  {li1 li2 li3} (cc12: callconv li1 li2) (cc23: callconv li2 li3):
+  Genv.symtbl * ccworld cc12 * ccworld cc23 ->
+  forall sk1 sk3, Genv.skel_path sk1 sk3 -> Genv.symtbl -> Genv.symtbl -> Prop :=
+  | Match_senv_compose_intro se1 se2 se3 sk1 sk2 sk3 w12 w23
+      (path12: Genv.skel_path sk1 sk2) (path23: Genv.skel_path sk2 sk3)
+      (SE12: match_senv cc12 w12 path12 se1 se2)
+      (SE23: match_senv cc23 w23 path23 se2 se3):
+      match_senv_compose cc12 cc23 (se2, w12, w23)
+        sk1 sk3 (Genv.Compose path12 path23) se1 se3.
 
 Program Definition cc_compose {li1 li2 li3} (cc12: callconv li1 li2) (cc23: callconv li2 li3) :=
   {|
     ccworld := Genv.symtbl * ccworld cc12 * ccworld cc23;
-    match_senv w se1 se3 se_path := match_senv_compose cc12 cc23 w se_path;
+    valid_skel := valid_skel_compose cc12 cc23;
+    match_senv w := match_senv_compose cc12 cc23 w;
     match_query '(se2, w12, w23) q1 q3 :=
       exists q2,
         match_query cc12 w12 q1 q2 /\
@@ -115,13 +138,14 @@ Program Definition cc_compose {li1 li2 li3} (cc12: callconv li1 li2) (cc23: call
         match_reply cc12 w12 r1 r2 /\
         match_reply cc23 w23 r2 r3;
   |}.
-(* Next Obligation. *)
-(*   intros. rename sk2 into sk3. rename se2 into se3. *)
-(*   destruct w as [[se2 w12] w23]. inv H. *)
-(*   apply match_senv_local in SE12. *)
-(*   apply match_senv_local in SE23. *)
-(*   eapply Genv.valid_stbls_compose; eauto. *)
-(* Qed. *)
+Next Obligation.
+  intros. rename sk2 into sk3. rename se2 into se3.
+  destruct w as [[se2 w12] w23]. inv H. inv H0.
+  subst_dep.
+  apply match_senv_local in SE12; eauto.
+  apply match_senv_local in SE23; eauto.
+  eapply Genv.valid_stbls'_compose; eauto.
+Qed.
 
 Infix "@" := cc_compose (at level 30, right associativity) : cc_scope.
 
@@ -173,10 +197,14 @@ Inductive cc_c_reply R (w: world R): relation c_reply :=
       match_mem R w m1' m2' ->
       cc_c_reply R w (cr vres1 m1') (cr vres2 m2').
 
+(* TODO: for most passes we use [valid_skel_id], but for Unusedglob, we need
+   something more general *)
 Program Definition cc_c (R: cklr): callconv li_c li_c :=
   {|
     ccworld := world R;
-    match_senv w se1 se2 _se_path := match_stbls R w se1 se2;
+    valid_skel _ _ path := valid_skel_id path;
+    match_senv w sk1 sk2 _sk_path se1 se2 :=
+      match_stbls R w se1 se2 /\ Genv.valid_stbls' sk1 sk2 se1 se2;
     match_query := cc_c_query R;
     match_reply := (<> cc_c_reply R)%klr;
   |}.
